# 统计推断

[lecture 1-2](%E7%BB%9F%E8%AE%A1%E6%8E%A8%E6%96%AD%2058317d0da28d4cc59f3e35399698b895/lecture%201-2%2059aa04c4f6904cdfadd93854d591771a.md)

[lecture 3-4](%E7%BB%9F%E8%AE%A1%E6%8E%A8%E6%96%AD%2058317d0da28d4cc59f3e35399698b895/lecture%203-4%209ae98cbdebec4af4a1301b7bdad758fe.md)

[lecture 5-6](%E7%BB%9F%E8%AE%A1%E6%8E%A8%E6%96%AD%2058317d0da28d4cc59f3e35399698b895/lecture%205-6%209c1e838f719d4f1487b2e03f7e61953c.md)

[lecture 7-8](%E7%BB%9F%E8%AE%A1%E6%8E%A8%E6%96%AD%2058317d0da28d4cc59f3e35399698b895/lecture%207-8%204635c9e0be5b466f8117bf8487c9d08b.md)

[lecture 9-10](%E7%BB%9F%E8%AE%A1%E6%8E%A8%E6%96%AD%2058317d0da28d4cc59f3e35399698b895/lecture%209-10%20acf4394130eb4bc488640b4ca6e49a2f.md)

[lecture 11-12](%E7%BB%9F%E8%AE%A1%E6%8E%A8%E6%96%AD%2058317d0da28d4cc59f3e35399698b895/lecture%2011-12%209a3c57e981744adb91ba6a7bf9181b88.md)

[lecture 13-14](%E7%BB%9F%E8%AE%A1%E6%8E%A8%E6%96%AD%2058317d0da28d4cc59f3e35399698b895/lecture%2013-14%20d73b680e0a704d58a7ff517dba01e6e0.md)

一些常用技术

1. **取补**

e.g. Proof of mean square error   $MSE= Var(\hat{\theta})+[E(\hat{\theta})-\theta]^2$

$Proof.$ 

$$
\begin{split}
E[({\theta-\hat{\theta})^2}]&=E[(\theta-E(\hat{\theta})+E(\hat{\theta})-\hat{\theta})^2]\\
&=E[(\theta-E(\hat{\theta}))^2]+E[(\hat{\theta}-E(\hat{\theta}))^2]+2E[(\theta-E(\hat{\theta}))(E(\hat{\theta})-\hat{\theta})]\\
&=Var(\hat{\theta})+[E(\hat{\theta})-\theta]^2, \ where \ \theta-E(\hat\theta) \in C
\end{split} 
$$

1. **标准均匀分布的一些结论**

If X~ U(0,1), then $f(x_{(k)})=\frac{n!}{(k-1)!(n-k)!}x^{k-1}(1-x)^{n-k}$, thus $X_{(k)} \sim Be(k,n-k+1)$

for $(Y,Z)=(X_{(1)},X_{(n)}),$ $f(y,z)=n(n-1)(z-y)^{n-2}$

also for R=Z-Y, we have $f(r)=n(n-1)r^{n-2}(1-r), \ 0<r<1,\ R \sim Be(n-1,2)$

1. **三大分布的一些结论**

1. 卡方分布: 标准正态分布的平方的和

- $\bar{x}$ 与 $s^2$ 独立
- $(n-1)s^2/\sigma^2 \sim \chi^2(n-1)$

1. fisher distribution: 分子分母的卡方分布除以自由度
- $\frac{s_x^2/\sigma^2_1}{s^2_y/\sigma^2_2} \sim F(m-1,n-1)$
- $F_\alpha(n, m)=1/ F_{1-\alpha}(m,n)$

$proof.$

Note that if $F \sim F(n,m)$, then $1/F \sim F(m,n)$. Let $\alpha := P(F \leq F_\alpha(n, m)) =P(1/F \geq 1/F_\alpha(n, m))$

Hence, we get $P(1/F \leq 1/F_\alpha(n, m))=1 - \alpha$, which implies 

$$
F_{1-\alpha}(m,n)=1/F_{\alpha}(n,m) \iff F_\alpha(n,m)=1/F_{1-\alpha}(m,n)
$$

1. t distribution: $t=X_1/\sqrt{X_2/n}$ , $X_1 \sim N(0,1)$, $X_2 \sim \chi^2(n)$
- $(\bar{x}- \mu)/(s/\sqrt{n}) \sim t(n-1)$, also

$$
\frac{(\bar{x}-\bar{y})-(\mu_1-\mu_2)}{s_w\sqrt{1/m+1/n}} \sim t(m+n-2)
$$

where

$$
s^2_w=\frac{(m-1)s^2_x+(n-1)s^2_y}{m+n-2}
$$

$proof:$

The proof follows similar arguments above. 

First, we note that 

$$
\frac{(\bar{x}-\bar{y})-(\mu_1-\mu_2)}{\sigma\sqrt{1/m+1/n}} \sim N(0,1)
$$

also,

$$
\frac{(m+n-2)s^2_w}{\sigma^2} \sim \chi^2(m+n-2)
$$

As $\bar{x}$ is independent to $s_x^2$, and $\bar{y}$ is independent to $s_y^2$, or they are mutually independent, then $\bar{x}-\bar{y}$ is independent to $s_w^2$.

Thus, by definition of t distribution, we get what we want.    $\Box$